code/chacha20/Hacl.Chacha20.Vec32.fst
@@ -1,0 +1,15 @@
+module Hacl.Chacha20.Vec32
+
+open FStar.HyperStack
+open FStar.HyperStack.All
+
+open Lib.IntTypes
+open Lib.Buffer
+
+open Hacl.Impl.Chacha20.Vec
+
+let chacha20_encrypt : chacha20_encrypt_st 1 =
+  chacha20_encrypt
+
+let chacha20_decrypt : chacha20_decrypt_st 1 =
+  chacha20_decrypt
